Renamed files; moved old files to detritus directory.

Refinement.v
@@ -1,61 +1,70 @@
-
 Require Import Bool.
 Require Import Heap.
 
 Definition S := heap.
 
-Definition Pow : Type -> Type := fun a => a -> Prop.
+Definition Pow : Type -> Type := fun a => a -> Type.
 
-Definition K : forall {A}, Pow S -> (forall s:S, A s -> Pow S) := fun a pt _ _ s => pt s.
+Definition K : forall {A} {a : Type}, Pow S -> (forall s:S, A s -> a -> Pow S) := fun a _ pt _ _ _ s => pt s.
+
+Definition Ka : forall {A} {a : Type}, (a -> Pow S) -> (forall s:S, A s -> a -> Pow S) := fun _ _ pt _ _ a s => pt a s.
 
 Implicit Arguments K [A].
 
-Definition subset : Pow S -> Pow S -> Prop :=
+Implicit Arguments Ka [A].
+
+Definition subset : Pow S -> Pow S -> Type :=
   fun P1 P2 => forall s, P1 s -> P2 s.
 
 Notation "P1 ⊂ P2" := (subset P1 P2) (at level 80) : type_scope.
 
-Inductive PT : Type :=
-  Predicate : forall pre : Pow S, (forall s : S, pre s -> Pow S) -> PT.
+(* Extended PT to cover the return type  -- now the postcondition refers to the return value also *)
+Inductive PT (a : Type) : Type :=
+  Predicate : forall pre : Pow S, (forall s : S, pre s -> a -> Pow S) -> PT a.
 
-Definition pre (pt : PT) : Pow S := 
+Definition pre {a : Type} (pt : PT a) : Pow S := 
   match pt with
-    | Predicate pre _ => pre
+    | Predicate _ pre _ => pre
   end.
 
-Definition post (pt : PT) : (forall s : S, pre pt s -> Pow S) :=
-  match pt return (forall s : S, pre pt s -> Pow S) with
-    | Predicate _pre p => p
+Definition post {a : Type} (pt : PT a) : (forall s : S, pre pt s -> a -> Pow S) :=
+  match pt return (forall s : S, pre pt s -> a -> Pow S) with
+    | Predicate _ _pre p => p
   end.
 
-Definition extend (pt : PT) (U : Pow S) : Pow S := 
-  fun s => { p : pre pt s & post pt s p ⊂ U}.
-
-Inductive Refines (pt1 pt2 : PT) : Type :=
+Inductive Refines {a : Type} (pt1 pt2 : PT a) : Type :=
   Refinement : 
     forall (d : pre pt1 ⊂ pre pt2), 
-      (forall (s : S) (x : pre pt1 s), post pt2 s (d s x) ⊂ post pt1 s x) -> Refines pt1 pt2.
+      (forall (s : S) (x : pre pt1 s) v, post pt2 s (d s x) v ⊂ post pt1 s x v) -> Refines pt1 pt2.
+
+(* Joao: please double-check this definition *)
+(* Wouter: It's OK I think. The question is where you quantify the v. 
+I'd expect a predicate transformer on Pow (A*S) -> Pow (A*S)
+Does that make sense?
+*) 
+
+Definition extend {a : Type} (pt : PT a) (v : a) (U : Pow S) : Pow S
+  := fun s => { p : pre pt s & post pt s p v ⊂ U}.
 
 Notation "PT1 ⊏ PT2" := (Refines PT1 PT2) (at level 90, no associativity) : type_scope.
 
-Notation "[ p , q ]" := (Predicate p q) (at level 70) : type_scope.
+Notation "[ p , q ]" := (Predicate _ p q) (at level 70) : type_scope.
 
 Ltac refine_simpl := unfold subset, pre, post, extend; simpl; auto.
 
 (*** Structural laws ***)
 
-Lemma strengthenPost (P : Pow S) (Q1 Q2 : forall s, P s -> Pow S) :
-  (forall (s : S) (p : P s), Q1 s p ⊂ Q2 s p) -> 
+Lemma strengthenPost {a : Type} (P : Pow S) (Q1 Q2 : forall s, P s -> a -> Pow S) :
+  (forall (s : S) (p : P s) (v : a), Q1 s p v ⊂ Q2 s p v) -> 
   [ P , Q2 ] ⊏ [ P , Q1 ].
 Proof.
   intros.
   set (d := fun (s : S) (H: P s) => H).
   apply (Refinement ([P, Q2]) ([P, Q1]) d).
-  intros. unfold post. unfold pre in x. unfold subset in *. intros. apply H.
-  simpl in *; assumption.
+  intros. unfold post. unfold pre in x. unfold subset in *. intros. now auto.
 Qed.
 
-Lemma weakenPre (P1 P2 : Pow S) (f : P1 ⊂ P2) (Q : S -> Pow S) :
+Lemma weakenPre {a : Type} (P1 P2 : Pow S) (f : P1 ⊂ P2) (Q : S -> a -> Pow S) :
   [P1, fun s _ => Q s ] ⊏ [P2 , fun s _ => Q s ].
 Proof.
   intros.
@@ -65,413 +74,88 @@ Qed.
 
 (*** SKIP **)
 
-Definition Skip_PT : PT := 
+Definition SkipPT {a : Type} : PT a := 
   let skipPre := fun s => True in
-  let skipPost := fun s pres s' => s = s' in
+  let skipPost := fun s pres v s' => s = s' in
   [skipPre , skipPost].
 
 (* Law 4.1 *)
-Lemma refineSkip (pt : PT) : (forall s (pres : pre pt s), post pt s pres s) -> pt ⊏ Skip_PT.
+Lemma refineSkip {a : Type} (pt : PT a) :
+  (forall s (pres : pre pt s) v, post pt s pres v s) -> pt ⊏ SkipPT.
   Proof.
-    intros H; assert (d : pre pt ⊂ pre Skip_PT) by (unfold subset; simpl pre; auto).
-    apply (Refinement pt Skip_PT d).
-    simpl subset; intros s pres s' eq; rewrite <- eq; auto.
+    intros H; assert (d : pre pt ⊂ @pre a SkipPT) by (unfold subset; simpl pre; auto).
+    apply (Refinement pt SkipPT d).
+    simpl subset; intros s pres s' v eq; rewrite <- eq; auto.
   Qed.
-
-Lemma SkipExtendL (U : Pow S) : extend Skip_PT U ⊂ U.
-  Proof.
-    unfold extend; simpl subset; intros s [P1 P2]; apply P2; auto.
-  Qed.
-
-Lemma SkipExtendR (U : Pow S) : U ⊂ extend Skip_PT U.
-  Proof.
-    unfold extend, subset; intros s Us; simpl; split; [trivial | intros s' eq; rewrite <- eq; now trivial].
-  Qed.
-
 
 (*** ASSIGNMENT ***)
 
-Definition Assign_PT : (Pow S) -> (S -> S) -> PT := fun p f =>
+Definition AssignPT {a : Type} : (Pow S) -> (S -> S) -> PT a := fun p f =>
   let assignPre := p in
-  let assignPost := fun s _ s' => prod (s' = f s) (p s') in
+  let assignPost := fun s _ v s' => prod (s' = f s) (p s') in
   [assignPre , assignPost].
 
 (* Law 1.3 *)
-Lemma refineAssignPT (pt : PT) (p : Pow S) (f : S -> S) (h : forall (s : S) (pre : pre pt s),  post pt s pre (f s)) (h' : pre pt ⊂ p)
-  : pt ⊏ Assign_PT p f.
+Lemma refineAssignPT {a : Type} (pt : PT a) (p : Pow S) (f : S -> S) (h : forall (s : S) (pre : pre pt s) (v : a),  post pt s pre v (f s)) (h' : pre pt ⊂ p)
+  : pt ⊏ AssignPT p f.
   Proof.
-    assert (d : pre pt ⊂ pre (Assign_PT p f)); refine_simpl.
-    eapply (Refinement pt (Assign_PT p f) d).
-    simpl; intros s pres s' [eq p']; rewrite eq; auto.
+    assert (d : pre pt ⊂ @pre a (AssignPT p f)); refine_simpl.
+    eapply (Refinement pt (AssignPT p f) d).
+    simpl; intros s pres s' v' [eq p']; rewrite eq; auto.
   Qed.
 
-(*
-Lemma AssignExtendL (U : Pow S) (p : Pow S) (f : S -> S) (s : S) 
-  : extend (Assign_PT p f) U s -> U (f s).
-  Proof.
-    unfold extend; intros [H1 H2]; apply H2. reflexivity.
-  Qed.
-
-
-Lemma AssignExtendR  (U : Pow S) (p : Pow S) (f : S -> S) (s : S) 
-  : U (f s) -> extend (Assign_PT p f) U s.
-  Proof.
-    intros Ufs; unfold extend; simpl; split; [ trivial | unfold subset; intros s' eq; rewrite eq; now trivial].
-  Qed.
-*)
-
-(*** SEQUENCING **)
-
-Definition Seq_PT (pt1 pt2 : PT) : PT :=
-  let seqPre := fun s => {pres : pre pt1 s | forall t, post pt1 s pres t -> pre pt2 t} in
-  let seqPost : forall s : S, seqPre s -> Pow S := fun (s : S) (pres : seqPre s) (s' : S) => 
-    exists t : S, exists q : post pt1 s (proj1_sig pres) t, post pt2 t (proj2_sig pres t q) s'
+(*** SEQUENCING (ignoring return values) **)
+  
+Definition SeqPT {a : Type} (pt1 pt2 : PT a) : PT a :=
+  let seqPre := fun s => {pres : pre pt1 s & forall t v, post pt1 s pres v t -> pre pt2 t} in
+  let seqPost : forall s : S, seqPre s -> a -> Pow S := fun (s : S) (pres : seqPre s) (v : a) (s' : S) => 
+  { t : S & {
+    v : a & {
+    q : post pt1 s (projT1 pres) v t &
+    post pt2 t (projT2 pres t v q) v s'}}}
+  (* exists t : S, exists v, exists q : post pt1 s (projT1 pres) v t, post pt2 t (projT2 pres t v q) v s' *)
   in
   [seqPre , seqPost].
 
-Notation "pt1 ;; pt2" := (Seq_PT pt1 pt2) (at level 52, right associativity).
+Notation "pt1 ;; pt2" := (SeqPT pt1 pt2) (at level 52, right associativity).
+
+Definition BindPT {a b : Type} (pt1 : PT a) (pt2 : a -> PT b) : PT b :=
+  let seqPre := fun s => {pres : pre pt1 s & forall t v, post pt1 s pres v t -> pre (pt2 v) t} in
+               
+  let seqPost : forall s : S, seqPre s -> b -> Pow S := fun (s : S) (pres : seqPre s) (v : b) (s' : S) =>
+    {t : S & {
+     x : a & {
+     q : post pt1 s (projT1 pres) x t &
+     post (pt2 x) t (projT2 pres t x q) v s'}}}
+    (* exists t : S, exists x, exists q : post pt1 s (proj1_sig pres) x t, post (pt2 x) t (proj2_sig pres t x q) v s'*)
+  in
+  [seqPre , seqPost].
+
+(* 
+Notation "pt1 ⟫= pt2" := (Seq_PT pt1 pt2) (at level 52, right associativity).
+*)
 
 (* Law 4.2 *)
-Lemma refineSeqPT (Pre Mid Post : Pow S) :
-  let pt := [ Pre , fun _ _ s' => Post s' ] in
-  pt ⊏ ([Pre , (fun _ _ s' => Mid s') ] ;; [Mid , (fun _ _ s' => Post s') ]).
+Lemma refineSeqPT {a : Type} (Pre Mid Post : Pow S) :
+  let pt := [ Pre , fun _ _ v s' => Post s' ] in
+  pt ⊏ ([Pre , (fun _ _ v s' => Mid s') ] ;; [Mid , (fun _ _ (v : a) s' => Post s') ]).
   Proof.
     refine_simpl.
-    assert (d : pre (Predicate Pre (K Post)) ⊂ pre ([Pre , (K Mid) ] ;; [Mid , (K Post) ])); refine_simpl.
+    assert (d : pre (Predicate _ Pre (K a Post)) ⊂ pre ([Pre , (K _ Mid) ] ;; [Mid , (K a Post) ])); refine_simpl.
     intros s pres; exists pres; auto.
     eapply (Refinement _ _ d).
-    refine_simpl; intros s x s' H; destruct H as [t q]; destruct q; auto.
-  Qed.
-
-(*
-Lemma refineSeqAssignPT : forall (f: S -> S) (g: S -> S) (h: S -> S),
-  (forall (s : S), h s = g (f s)) -> 
-  Assign_PT h ⊏ Assign_PT f ;; Assign_PT g.
-Proof.
-  intros.
-  assert (d: pre (Assign_PT h) ⊂ pre (Assign_PT f ;; Assign_PT g)).
-  unfold Assign_PT,Seq_PT,subset; simpl.
-  intros; apply exist. 
-  assumption. 
-  intros; assumption.
-  apply (Refinement _ _ d).
-  simpl in *; unfold subset in *. 
-  intros; inversion H0; inversion H1; rewrite H.
-  rewrite <- x1; rewrite <- H2; reflexivity.
+    refine_simpl; intros s x v s' H; destruct H as [t [v' q]]; destruct q; auto.
 Qed.
-*) 
- 
-Lemma seqExtendL (pt1 pt2 : PT) (U : Pow S) (s : S) : 
-  extend pt1 (extend pt2 U) s -> extend (Seq_PT pt1 pt2) U s.
+
+(* Joao: does this look good? *)
+Lemma refineBindPT {a : Type} (Pre : Pow S) (Mid Post : a -> Pow S) :
+  let pt := [ Pre , fun _ _ v s' => Post v s' ] in
+  pt ⊏ BindPT ([Pre , (fun _ _ v s' => Mid v s') ]) (fun a => [ Mid a , (fun _ _ v s' => Post v s') ]).
   Proof.
     refine_simpl.
-    intro H; destruct H as [pres posts].
-    exists (exist (fun pres => forall t, post pt1 s pres t -> pre pt2 t) pres 
-             (fun t pt => projT1 (posts t pt))).
-    unfold subset in *; simpl.
-    intros s' H; destruct H as [s'' q]; destruct q as [H1 H2].
-    apply (projT2 (posts s'' H1)); auto.
-  Qed.
-
-Lemma seqExtendR (pt1 pt2 : PT)  (U : Pow S) (s : S) : 
-  extend (Seq_PT pt1 pt2) U s -> extend pt1 (extend pt2 U) s.
-  Proof.
-   unfold extend, subset; simpl; intro H; destruct H as [[pre1 pre2] post1].
-   exists pre1.
-   intros s' H; exists (pre2 s' H).
-   intros s'' post3; apply (post1 s''); exists s'; exists H; exact post3.
-  Qed.
-
-
-(*** CONDITIONALS ***)
-
-Definition Is_false (b : bool) :=
-  match b with
-    | true => False
-    | false => True
-  end.
-
-Definition If_PT (cond : S -> bool) (Then Else : PT) : PT :=
-  let ifPre := fun s => 
-    prod (Is_true (cond s) -> pre Then s)
-         (Is_false (cond s) -> pre Else s)
-  in
-  let ifPost := fun s pres s' => 
-    prod (forall (p : Is_true (cond s)), post Then s (fst pres p) s') 
-         (forall (p : Is_false (cond s)), post Else s (snd pres p) s')
-  in
-  [ ifPre , ifPost ].
-
-Lemma refineIfPT' (cond : S -> bool) (pt : PT) :
-  pt ⊏ If_PT cond pt pt.
-  Proof.
-    set (d (s : S) (X : pre pt s) := 
-      (fun H : Is_true (cond s) => X, fun H : Is_false (cond s) => X)).
-    apply (Refinement pt (If_PT cond pt pt) d).
-    unfold subset; simpl; intros.
-    destruct H as [ T F ].
-    assert (Ha : forall p, Is_true p \/ Is_false p) by 
-    (intros; destruct p; [ left; unfold Is_true; trivial | right; unfold Is_false; trivial ]).
-    assert (Ha' : Is_true (cond s) \/ Is_false (cond s)) by (apply Ha).
-    inversion Ha'; [ apply T; assumption | apply F; assumption ].
+    assert (d : pre (Predicate _ Pre (Ka _ Post)) ⊂ pre (BindPT ([Pre, Ka _ Mid])
+       (fun v => [Mid v, Ka _ Post]))); refine_simpl.
+    intros s pres; exists pres; auto.
+    eapply (Refinement _ _ d).
+    refine_simpl; intros s x v s' H; destruct H as [t [v' q]]; destruct q; auto.
 Qed.
-
-(* Law 5.1 *)
-Lemma refineIfPT (cond : S -> bool) (pt : PT) :
-  let branchPre (P : S -> Prop) := fun s => prod (pre pt s) (P s) in
-  let thenBranch := [branchPre (fun s => Is_true (cond s)),
-                     fun s pre s' => post pt s (fst pre) s' ] in
-  let elseBranch := [branchPre (fun s => Is_false (cond s)),
-                     fun s pre s' => post pt s (fst pre) s' ] in
-  pt ⊏ If_PT cond thenBranch elseBranch.
-  Proof.
-    intros.
-    set (d (s : S) (X : pre pt s) := 
-      (fun H : Is_true (cond s) => (X,H), fun H : Is_false (cond s) => (X,H))).
-    apply (Refinement pt (If_PT cond thenBranch elseBranch) d).
-    simpl; intros s pres s'; destruct (cond s); simpl; intros [H3 H4];  auto.
-  Qed.
-
-Lemma IfExtendL (cond : S -> bool) (thenPt elsePt : PT) (U : Pow S) (s : S) :
-  extend (If_PT cond thenPt elsePt) U s ->
-    (Is_true (cond s) -> extend thenPt U s) * (Is_false (cond s) -> extend elsePt U s).
-  Proof.
-    unfold extend; simpl; destruct (cond s); simpl; split; try contradiction;
-      unfold subset in *; simpl in *; destruct H as [[Pre1 Pre2] Post].
-    intros; exists (Pre1 I);
-      intros s' H'; apply Post; split; simpl; intros; destruct p; assumption.
-    intros; exists (Pre2 I);
-      intros s' H'; apply Post; split; simpl; intros; destruct p; assumption.
-  Qed.
-
-Lemma IfExtendR (cond : S -> bool) (thenPt elsePt : PT) (U : Pow S) (s : S) :
-    (Is_true (cond s) -> extend thenPt U s) * (Is_false (cond s) -> extend elsePt U s) ->
-    extend (If_PT cond thenPt elsePt) U s.
-  Proof.
-  unfold extend, subset. simpl; case (cond s); simpl; intros [H1 H2];
-  exists (fun t => projT1 (H1 t) , fun f => projT1 (H2 f)).
-    intros; apply (projT2 (H1 I)); destruct H as [A _]; apply A.
-    intros; apply (projT2 (H2 I)); destruct H as [_ A]; apply A.
-  Qed.
-
-Definition While_PT (inv : Pow S) (cond : S -> bool) (body : PT) : PT :=
-  let whilePre := (fun s =>   (* The invariant should hold initially *)
-                             inv s /\ 
-                              (* If we enter the loop, the precondition of the body should hold *)
-                            { H : (forall s, Is_true (cond s) /\ inv s -> pre body s) &
-                              (* The loop body should preserve the invariant *)
-                            (forall s s' (t : Is_true (cond s) /\ inv s), post body s (H s t)  s' -> inv s')})                          
-  in
-  let whilePost := (fun _ _ s' => inv s' /\ Is_false (cond s')) in
-  [ whilePre , whilePost ].
-
-(* Law 7.1 *)
-Lemma refineWhilePT (inv : Pow S) (cond : S -> bool) (Q : Pow S) : 
-  let pt := [inv , fun _ _ s' => inv s' /\ Q s'] in
-  let body := [fun s => inv s /\ Is_true (cond s), (fun _ _ s => inv s)] in
-  (forall s, Is_false (cond s) -> Q s) ->
-  pt ⊏ While_PT inv cond body.
-  Proof.
-    intros pt body QH; simpl in *.
-    assert (d: pre pt ⊂ pre (While_PT inv cond body)).
-    unfold subset, pt,While_PT; simpl; intros; split; [assumption | ].
-    split.
-    intros s' H1. 
-    destruct H1; split; assumption.
-    intros s' s'' [H1 H2] H3; assumption.
-    apply (Refinement _ _ d).
-    intros s PreS s' [H1 H2].
-    split; [ | apply QH]; assumption.
-Qed.
-
-Definition WhileSemantics  (inv : Pow S) (cond : S -> bool) (body : PT) (U : Pow S) (s : S) : Type
-  := inv s 
-    /\ (forall s, Is_true (cond s) /\ inv s -> extend body inv s)
-    /\ (forall s, Is_false (cond s) /\ inv s -> U s).
-
-Lemma WhileExtendL (inv : Pow S) (cond : S -> bool) (body : PT) (U : Pow S) (s : S) :
-  extend (While_PT inv cond body) U s -> WhileSemantics inv cond body U s.
-  Proof.
-    unfold extend; simpl; intros [[H1 [H2 H3] H4 ]].
-    split; [ assumption | split].
-    - intros s' [H5 H6].
-      unfold extend; exists (H2 s' (conj H5 H6)); intros s'' H7; eapply H3; exact H7.
-    - intros s' [A B]; apply H4; split; try assumption.
-  Qed.
-
-Lemma WhileExtendR (inv : Pow S) (cond : S -> bool) (body : PT) (U : Pow S) (s : S) :
-  WhileSemantics inv cond body U s ->
-    extend (While_PT inv cond body) U s.
-  Proof.
-    unfold extend; intros [I [T F]]; simpl in *.
-    split; [split; [assumption | ] | ].
-    set (H := fun s Hs => projT1 (T s Hs)); exists H.
-    intros; eapply (projT2 (T s0 t)); unfold H in *; assumption.
-    intros s' [H1 H2]; apply F; split; assumption.
-Qed.
-
-Definition refineTransPT (pt2 pt1 pt3 : PT) : 
-  pt1 ⊏ pt2 -> pt2 ⊏ pt3 -> pt1 ⊏ pt3.
-    intros [pre12 post12] [pre23 post23].
-    set (d (s : S) (pre1s : pre pt1 s) := pre23 s (pre12 s pre1s)).
-    refine (Refinement pt1 pt3 d _).
-    intros s pres s' post3.
-    apply post12; apply post23; auto.
-  Defined.
-
-Definition refineReflPT (pt : PT) : pt ⊏ pt.
-  refine (Refinement pt pt (fun s pres => pres) _).
-  intros; unfold subset; auto.
-  Defined.
-
-Definition refineSplitPT (pt1 pt2 pt3 pt4 : PT) :
-  (pt1 ⊏ pt3) -> (pt2 ⊏ pt4) -> (pt1 ;; pt2) ⊏ (pt3 ;; pt4).
-    intros  [d1 f1] [d2 f2].
-    set (d (s : S) (pres : pre (pt1;; pt2) s) :=
-          exist (fun pres0 : pre pt3 s => forall t : S, post pt3 s pres0 t -> pre pt4 t)
-          (d1 s (proj1_sig pres))
-          (fun (t : S) (post2 : post pt3 s (d1 s (proj1_sig pres)) t) =>
-            d2 t (proj2_sig pres t (f1 s (proj1_sig pres) t post2))) : pre (pt3;;pt4) s 
-      ).
-    apply (Refinement _ _ d).
-    unfold d in *.
-    simpl; intros s Pre s' [t [P Q]].
-    exists t. exists (f1 s (proj1_sig Pre) t P).
-    apply f2; auto.
-  Defined.
-
-Definition refineSplitIfPT (pt1 pt2 pt3 pt4 : PT) (cond : S -> bool) :
-  (pt1 ⊏ pt3) -> (pt2 ⊏ pt4) -> If_PT cond pt1 pt2 ⊏ If_PT cond pt3 pt4.
-  intros [d1 f1] [d2 f2].
-  set (d (s : S) (X : pre (If_PT cond pt1 pt2) s)
-         := (fun C : Is_true (cond s) => d1 s (fst X C),
-             fun C : Is_false (cond s) => d2 s (snd X C)) 
-            : pre (If_PT cond pt3 pt4) s).
-  apply (Refinement _ _ d).    
-  simpl; intros s pres s' [H1 H2].
-  split; intros; [apply f1; apply H1 | apply f2; apply H2]; auto.
-  Defined.
-
-Lemma refineBodyPT : forall (inv : Pow S) (cond : S -> bool) (bodyL bodyR : PT),
-  bodyL ⊏ bodyR ->
-  While_PT inv cond bodyL ⊏ While_PT inv cond bodyR.
-Proof.
-  intros inv cond bodyL bodyR [Pre Post].
-  assert (a: pre (While_PT inv cond bodyL) ⊂ pre (While_PT inv cond bodyR)).
-  unfold subset; simpl; intros s [Inv [H1 H2]]; split.
-  assumption.
-  (* assert (E:  forall s0 : S, Is_true (cond s0) /\ inv s0 -> pre bodyR s0). *)
-  set (E := fun s0 H => Pre s0 (H1 _ H)).
-  exists E.
-  intros s0 s' P Q.
-  eapply H2.
-  apply Post.
-  unfold E in Q.
-  exact Q.
-
-  apply (Refinement _ _ a).
-  intros.
-  unfold post,subset,While_PT in *.
-  simpl in *.
-  intros; assumption.
-Qed.
-
-Lemma refineSeqAssocR_PT_pre : forall (pt1 pt2 pt3 : PT),
-  pre ((pt1 ;; pt2) ;; pt3) ⊂ pre (pt1;; pt2;; pt3).
-Proof.
-  unfold subset; simpl; intros.
-  destruct H as [[H1 H2] H3].
-  exists H1.
-  intros.
-  simpl in H3.
-  eexists.
-  intros u H4.
-  apply H3.
-  exists t.
-  exists H.
-  exact H4.
-Defined.
-
-Lemma refineSeqAssocR_PT : forall (pt1 pt2 pt3 : PT),
-  ((pt1 ;; pt2) ;; pt3) ⊏ (pt1 ;; pt2 ;; pt3).
-Proof.
-  intros.
-  apply (Refinement _ _ (refineSeqAssocR_PT_pre _ _ _)).
-  refine_simpl.
-  intros.
-  destruct H as [t [q [t' [q' H]]]].
-  exists t'.
-  repeat destruct x; simpl in *.
-  exists (ex_intro _ t (ex_intro _ q q')).
-  exact H.
-Defined.
-
-(* Lemma refineSeqAssocL_PT_pre : forall (pt1 pt2 pt3 : PT), *)
-(*   pre (pt1 ;; pt2 ;; pt3) ⊂ pre ((pt1;; pt2);; pt3). *)
-(* Proof. *)
-(*   unfold subset; simpl; intros. *)
-(*   destruct H as [H1 H2]. *)
-(*   exists (exist _ _ (fun (t : S) (post1 : post pt1 s _ t) => match H2 t post1 with *)
-(*                                                              exist _ p h => p *)
-(*                                                              end)). *)
-(*   simpl. *)
-(*   intros t [t' [H3 H4]]. *)
-(*   destruct (H2 t' H3). *)
-(*   apply p. *)
-(*   exact H4. *)
-(* Defined. *)
-(*
-Lemma refineSeqAssocL_PT : forall (pt1 pt2 pt3 : PT),
-  (pt1 ;; pt2 ;; pt3) ⊏ ((pt1 ;; pt2) ;; pt3).
-Proof.
-  intros.
-  apply (Refinement _ _ (refineSeqAssocL_PT_pre _ _ _)).
-  refine_simpl.
-  intros s x s' H.
-  destruct H as [t [[t' [p q]] r]].
-n  exists t'.
-  repeat destruct x; simpl in *.
-  exists p.
-  exists t.
-  exists q.
-  destruct (s0 t' p).
-  simpl in *.
-  exact r.
-Defined.
-*)
-Lemma refineIfPT'' (cond : S -> bool) (pt : PT) (PThen PElse : Pow S) :
-  let branchPre (P : S -> Prop) := fun s => prod (pre pt s) (P s) in
-  let thenBranch := [branchPre PThen
-                    , fun s pre s' => post pt s (fst pre) s' ] in
-  let elseBranch := [branchPre PElse ,
-                     fun s pre s' => post pt s (fst pre) s'  ] in
-  let thenBranchBool := [branchPre (fun s => Is_true (cond s)), 
-                                     (fun s pre s' => post pt s (fst pre) s')] in
-  let elseBranchBool := [branchPre (fun s => Is_false (cond s)), 
-                                   (fun s pre s' => post pt s (fst pre) s')] in
-  (forall s : S, Is_true (cond s) -> PThen s) ->
-  (forall s : S, Is_false (cond s) -> PElse s) ->
-  pt ⊏ If_PT cond thenBranch elseBranch.
-  Proof.
-    intros.
-    rename H into H1; rename H0 into H2.
-    apply (refineTransPT (If_PT cond thenBranchBool elseBranchBool)).
-
-    set (d (s : S) (X : pre pt s) := 
-      (fun H : Is_true (cond s) => (X,H), fun H : Is_false (cond s) => (X,H))).
-    apply (Refinement pt (If_PT cond thenBranchBool elseBranchBool) d).
-    simpl; intros s pres s'; destruct (cond s); simpl; intros [H3 H4];  auto.
-
-    apply refineSplitIfPT.
-    set (d := (fun (s : S) (X : pre pt s * Is_true (cond s)) => 
-                   (fst X,H1 s (snd X))) : pre thenBranchBool ⊂ pre thenBranch).
-    apply (Refinement _ _ d).
-    unfold subset; intros.
-    simpl in *; assumption.
-
-    set (d := (fun (s : S) (X : pre pt s * Is_false (cond s)) => 
-                   (fst X,H2 s (snd X))) : pre elseBranchBool ⊂ pre elseBranch).
-    apply (Refinement _ _ d).
-    unfold subset; intros.
-    simpl in *; assumption.
-  Qed.
